commit

AP/Map/Defs.lean
@@ -1,14 +1,14 @@
 import AP.Util
 
 @[simp]
-def map_list_cnd.{u} {ι α : Type u} [LinearOrder ι] [DecidableEq α] : List (ι × α) → Prop
-| (x :: y :: xs) => x.1 < y.1 ∧ map_list_cnd (y :: xs)
+def Map.listCnd.{u} {ι α : Type u} [LinearOrder ι] [DecidableEq α] : List (ι × α) → Prop
+| (x :: y :: xs) => x.1 < y.1 ∧ Map.listCnd (y :: xs)
 | _ => True
 
 @[ext]
 structure Map.{u} (ι α : Type u) [LinearOrder ι] [DecidableEq α] : Type u where
-  xs : List (ι × α)
-  h : map_list_cnd xs
+  toList : List (ι × α)
+  h : Map.listCnd toList
 
 namespace Map
 
@@ -29,127 +29,11 @@ def insert' (x : ι × α) : List (ι × α) → List (ι × α)
   | .lt => x :: y :: xs
   | .gt => y :: insert' x xs
 
-omit hhα in
 @[simp]
-theorem insert'_nil {x : ι × α} : insert' x [] = [x] := rfl
+def ofList' (xs : List (ι × α)) : List (ι × α) → List (ι × α)
+| [] => xs
+| (y :: ys) => ofList' (insert' y xs) ys
 
-omit hhα in
-@[simp]
-theorem insert'_cons {x y : ι × α} {xs : List (ι × α)} :
-insert' x (y :: xs) = (match compare x.1 y.1 with
-| .eq => x :: xs
-| .lt => x :: y :: xs
-| .gt => y :: insert' x xs) := rfl
-
-theorem map_list_cnd_of_cons {x : ι × α} {xs}
-(h : map_list_cnd (x :: xs)) : map_list_cnd xs := by
-  cases xs; trivial; exact h.2
-
-theorem map_list_cnd_cons_of_congr {x y : ι × α} {xs}
-(h₁ : map_list_cnd (x :: xs)) (h₂ : x.1 = y.1) : map_list_cnd (y :: xs) := by
-  cases xs; trivial
-  nm z xs
-  simp at h₁ ⊢
-  rwa [←h₂]
-
--- #check 0 #exit
--- 
--- def insert_prod (mp : Map ι α) (x : ι × α) : Map ι α := by
---   use insert' x mp.xs
---   rcases mp with ⟨xs, h⟩
---   dsimp
---   induction xs
---   · simp
---   nm y xs ih
---   rcases y with ⟨j, y⟩
---   simp
---   split <;> nm x h₁ <;> clear x
---   · rw [compare_eq_iff_eq] at h₁
---     subst h₁
---     exact map_list_cnd_cons_of_congr h rfl
---   · rw [compare_lt_iff_lt] at h₁; simp; tauto
---   rw [compare_gt_iff_gt] at h₁
---   specialize ih # map_list_cnd_of_cons h
---   cases h₂ : insert' x xs
---   · simp
---   nm z zs
---   rw [h₂] at ih
--- 
--- #check 0 #exit
--- 
--- def insert_prod (p : ι × α) : Map ι α :=
---   mp.insert p.1 p.2
--- 
--- instance : Insert (ι × α) (Map ι α) :=
---   ⟨λ p mp => mp.insert_prod p⟩
--- 
--- def ofList' (mp : Map ι α) : List (ι × α) → Map ι α
--- | [] => mp
--- | (x :: xs) => (insert x mp).ofList' xs
--- 
--- def ofList : List (ι × α) → Map ι α :=
---   empty.ofList'
--- 
--- def lookup (i : ι) : Option α := by
---   obtain ⟨⟨s, hs⟩, h⟩ := mp
---   simp at h
---   apply s.lift_out λ xs => (xs.find? λ a => a.1 = i).map Prod.snd
---   intro xs ys hx hy
---   ext x
---   simp only [Option.map_eq_some_iff, List.find?_eq_some_iff_getElem, decide_eq_true_eq,
---     Bool.not_eq_eq_eq_not, Bool.not_true, decide_eq_false_iff_not, Prod.exists,
---     exists_eq_right, exists_eq_left]
---   change List.Perm _ _ at hx hy
---   have h₁ := hx.trans hy.symm
---   
---   have h₂ : (Quotient.out s).Nodup :=
---     by
---       unfold Multiset.Nodup at hs
---       generalize_proofs h₂ at hs
---       sorry
---   
---   have h₃ := List.Perm.nodup hx.symm h₂
---   have h₄ := List.Perm.nodup hy.symm h₂
---   
---   -- rw [List.perm_iff_count] at hx hy h₁
---   
---   constructor
---   · rintro ⟨n, hn, h₅, h₆⟩
---     have h₇ : xs[n] ∈ ys :=
---       by
---         rw [List.Perm.mem_iff (l₂ := xs)]
---         simp; exact h₁.symm
---     rw [List.mem_iff_getElem] at h₇
---     obtain ⟨n', hn', h₇⟩ := h₇
---     use n', hn', by rwa [h₇]
---     intro m' hm'
---     rw [List.nodup_iff_getElem?_ne_getElem?] at h₄
---     specialize h₄ m' n' hm' hn'
---     rw [List.getElem?_eq_getElem # by linarith] at h₄
---     rw [List.getElem?_eq_getElem # by linarith] at h₄
---     simp at h₄
---     contrapose! h₄
---     
---     have h₈ : ys[n'] ∈ s.out :=
---       by
---         rw [List.Perm.mem_iff (l₂ := ys)]
---         simp; exact hy.symm
---     have h₉ : ys[m'] ∈ s.out :=
---       by
---         rw [List.Perm.mem_iff (l₂ := ys)]
---         simp; exact hy.symm
---     rw [List.mem_iff_getElem] at h₈ h₉
---     obtain ⟨k₁, hk₁, h₈⟩ := h₈
---     obtain ⟨k₂, hk₂, h₉⟩ := h₉
---     
---     rw [←h₈]
---     rw [←h₉] at h₄ ⊢
---     specialize h i x
---     
---     sorry
---   
---   sorry
--- 
--- -- h₂ : ∀ (a b : List (ι × α)), (List.isSetoid (ι × α)) a b → a.Nodup = b.Nodup
--- -- hs : Quot.liftOn s List.Nodup h₂
--- -- ⊢ (Quotient.out s).Nodup
+def lookup' (i : ι) : List (ι × α) → Option α
+| [] => none
+| ((j, x) :: xs) => if i == j then some x else lookup' i xs
