AP/Map/Basic.lean
@@ -6,3 +6,190 @@ set_option linter.unusedVariables false
 universe u
 variable {ι α : Type u} [hhι : LinearOrder ι] [hhα : DecidableEq α] {mp : Map ι α}
 set_option linter.unusedSectionVars true
+
+omit hhα in
+@[simp]
+theorem insert'_nil {x : ι × α} : insert' x [] = [x] := rfl
+
+omit hhα in
+@[simp]
+theorem insert'_cons {x y : ι × α} {xs : List (ι × α)} :
+insert' x (y :: xs) = (match compare x.1 y.1 with
+| .eq => x :: xs
+| .lt => x :: y :: xs
+| .gt => y :: insert' x xs) := rfl
+
+theorem listCnd_of_cons {x : ι × α} {xs}
+(h : listCnd (x :: xs)) : listCnd xs := by
+  cases xs; trivial; exact h.2
+
+theorem listCnd_cons_of_le {x y : ι × α} {xs}
+(h₁ : listCnd (x :: xs)) (h₂ : y.1 ≤ x.1) : listCnd (y :: xs) := by
+  cases xs
+  · simp
+  nm z xs
+  simp at h₁ ⊢
+  rcases h₁ with ⟨h₁, h₃⟩
+  simp [h₃]
+  exact lt_of_le_of_lt h₂ h₁
+
+theorem listCnd_cons_of_eq {x y : ι × α} {xs}
+(h₁ : listCnd (x :: xs)) (h₂ : y.1 = x.1) : listCnd (y :: xs) := by
+  apply listCnd_cons_of_le h₁; rw [h₂]
+
+theorem listCnd_cons_of_lt {x y : ι × α} {xs}
+(h₁ : listCnd (x :: xs)) (h₂ : y.1 < x.1) : listCnd (y :: xs) := by
+  apply listCnd_cons_of_le h₁; exact le_of_lt h₂
+
+theorem listCnd_map_of {β : Type u} [hb : DecidableEq β] (f : α → β)
+{xs : List (ι × α)} (h : listCnd xs) :
+listCnd # xs.map # λ x => (x.1, f x.2) := by
+  induction xs
+  · simp
+  nm x xs ih
+  specialize ih # listCnd_of_cons h
+  cases xs <;> simp
+  nm y xs
+  simp at h ih
+  use h.1
+
+theorem listCnd_insert'_of {xs : List (ι × α)} {x}
+(h : listCnd xs) : listCnd (insert' x xs) := by
+  rcases x with ⟨i, x⟩
+  generalize hn : xs.length = n
+  induction n using Nat.strong_induction_on generalizing i x xs
+  nm n ih
+  cases xs
+  · simp
+  nm y xs
+  rcases y with ⟨j, y⟩
+  simp
+  split <;> nm a h₁ <;> clear a
+  · rw [compare_eq_iff_eq] at h₁
+    subst h₁
+    exact listCnd_cons_of_eq h rfl
+  · rw [compare_lt_iff_lt] at h₁
+    simp
+    use h₁
+  rw [compare_gt_iff_gt, gt_iff_lt] at h₁
+  simp at hn
+  have h₂ := ih (n - 1)
+  rw [←hn] at h₂
+  specialize @h₂ (by simp) xs (listCnd_of_cons h) i x (by simp)
+  generalize hy : insert' (i, x) xs = ys at h₂ ⊢
+  cases ys
+  · simp
+  nm z ys
+  simp [h₂]
+  cases xs
+  · simp at hy
+    simpa [←hy.1]
+  nm r xs
+  simp at h hy
+  split at hy <;> nm a h₃ <;> clear a <;>
+    simp at hy <;> rcases hy with ⟨rfl, hy⟩
+  · rw [compare_eq_iff_eq] at h₃
+    subst h₃
+    exact h.1
+  · rw [compare_lt_iff_lt] at h₃
+    exact h₁
+  exact h.1
+
+def insert_prod (x : ι × α) (mp : Map ι α) : Map ι α :=
+  ⟨_, listCnd_insert'_of (x := x) mp.h⟩
+
+instance : Insert (ι × α) (Map ι α) :=
+  ⟨λ p mp => mp.insert_prod p⟩
+
+@[simp]
+def insert (i : ι) (x : α) (mp : Map ι α) : Map ι α :=
+  mp.insert_prod (i, x)
+
+theorem listCnd_ofList'_of {xs ys : List (ι × α)}
+(h : listCnd xs) : listCnd (ofList' xs ys) := by
+  induction ys generalizing xs
+  · simpa
+  nm y ys ih
+  exact ih # listCnd_insert'_of h
+
+@[simp]
+theorem listCnd_ofList'_of_fst_nil {xs : List (ι × α)} :
+listCnd (ofList' [] xs) := by
+  apply listCnd_ofList'_of; simp
+
+def ofList (xs : List (ι × α)) : Map ι α :=
+  ⟨_, listCnd_ofList'_of_fst_nil (xs := xs)⟩
+
+def lookup (i : ι) (mp : Map ι α) : Option α :=
+  lookup' i mp.toList
+
+theorem lt_of_listCnd_cons_and_mem {xs : List (ι × α)} {x y}
+(h₁ : listCnd (x :: xs)) (h₂ : y ∈ xs) : x.1 < y.1 := by
+  generalize hn : xs.length = n
+  induction n using Nat.strong_induction_on generalizing x y xs
+  nm n ih
+  cases xs
+  · simp at h₂
+  nm z xs
+  simp at h₁
+  rcases h₁ with ⟨h₁, h₃⟩
+  simp at h₂
+  rcases h₂ with rfl | h₂
+  · exact h₁
+  specialize @ih (n - 1)
+  rw [←hn] at ih
+  apply @ih (by simp) xs x y _ h₂ (by simp)
+  exact listCnd_cons_of_lt h₃ h₁
+
+theorem listCnd_cons_of_forall_le {xs : List (ι × α)} {x}
+(h₁ : listCnd xs) (h₂ : ∀ y ∈ xs, x.1 < y.1) : listCnd (x :: xs) := by
+  cases xs
+  · simp
+  nm z xs
+  simp [h₁]
+  specialize h₂ z
+  simp at h₂
+  exact h₂
+
+theorem listCnd_cons_iff {xs : List (ι × α)} {x} :
+listCnd (x :: xs) ↔ listCnd xs ∧ ∀ y ∈ xs, x.1 < y.1 := by
+  use λ h => ⟨listCnd_of_cons h, λ _ => lt_of_listCnd_cons_and_mem h⟩
+  use λ h => listCnd_cons_of_forall_le h.1 h.2
+
+theorem sorted_of_listCnd {xs : List (ι × α)}
+(h : listCnd xs) : xs.Sorted # λ (x y : ι × α) => x.1 < y.1 := by
+  induction xs
+  · simp
+  nm x xs ih
+  specialize ih # listCnd_of_cons h
+  rw [List.sorted_cons]
+  simp only [ih, and_true]
+  intro y hy
+  exact lt_of_listCnd_cons_and_mem h hy
+
+theorem listCnd_of_sorted {xs : List (ι × α)}
+(h : xs.Sorted # λ (x y : ι × α) => x.1 < y.1) : listCnd xs := by
+  induction xs
+  · simp
+  nm x xs ih
+  rw [List.sorted_cons] at h
+  rcases h with ⟨h₁, h₂⟩
+  specialize ih h₂
+  rw [listCnd_cons_iff]
+  use ih
+
+theorem listCnd_iff_sorted {xs : List (ι × α)} :
+listCnd xs ↔ xs.Sorted (λ (x y : ι × α) => x.1 < y.1) :=
+  ⟨sorted_of_listCnd, listCnd_of_sorted⟩
+
+theorem nodup_of_listCnd {xs : List (ι × α)} (h : listCnd xs) : xs.Nodup := by
+  induction xs
+  · simp
+  nm x xs ih
+  specialize ih # listCnd_of_cons h
+  simp [ih]
+  rw [listCnd_cons_iff] at h
+  replace h := h.2
+  intro hx
+  specialize h x hx
+  simp at h
